proof/examples/zk/W64_exp_proof_5.ec
@@ -1,0 +1,127 @@
+require import AllCore IntDiv CoreMap List.
+
+require import JModel.
+require import BitEncoding.
+import BS2Int.
+
+require import Fp_small.
+require import Fp_small_proof.
+require import W64_exp_proof_1.
+require import W64_exp_proof_2.
+require import W64_exp_proof_3.
+require import W64_exp_proof_4.
+
+import Zp.
+import IterOp.
+
+
+
+
+module M5 = {
+
+    proc expm' (x:W64.t, n:W64.t) : W64.t = {
+    
+    var x1, x2, x3, x4, bit, d, p, par : W64.t;
+    var ctr:int;
+
+    d <- ith_bitword64 n (W64.size - 1);
+    (x1,x2,x3) <- (W64.one,W64.one,x);
+    x4 <@ ASpecFp.mulmw64(x,x);
+
+    ctr <- W64.size - 1;
+    p <- d;
+    (x1,x3) <- as_bool d ? (x3,x1) : (x1,x3);
+    (x2,x4) <- as_bool d ? (x4,x2) : (x2,x4);
+
+    while (0 < ctr) {
+      ctr <- (ctr - 1);
+      p <- d;
+      d <-  d `|` ith_bitword64 n ctr;
+      par <- ith_bitword64 n (ctr + 1) `^` ith_bitword64 n ctr;
+      (x1,x2) <- if as_bool par then (x2,x1) else (x1, x2);
+      x1 <@ ASpecFp.mulmw64(x1,x2); 
+      x2 <@ ASpecFp.mulmw64(x2,x2);  
+      (x1,x3) <- as_bool (d `^` p) ? (x3,x1) : (x1,x3);
+      (x2,x4) <- as_bool (d `^` p)  ? (x4,x2) : (x2,x4);
+    }
+    (x1,x2) <- if ! as_bool (ith_bitword64 n 0)  then (x2,x1) else (x1, x2);    
+    return x1;
+  }  
+
+    proc expm (m : W64.t, x:W64.t, n:W64.t) : W64.t = {
+    
+    var x1, x2, x3, x4, bit, d, p, par : W64.t;
+    var ctr:int;
+
+    d <- ith_bitword64 n (W64.size - 1);
+    (x1,x2,x3) <- (W64.one,W64.one,x);
+    x4 <@ M.mulm(m,x,x);
+
+    ctr <- W64.size - 1;
+    p <- d;
+    (x1,x3) <- as_bool d ? (x3,x1) : (x1,x3);
+    (x2,x4) <- as_bool d ? (x4,x2) : (x2,x4);
+
+    while (0 < ctr) {
+      ctr <- (ctr - 1);
+      p <- d;
+      d <-  d `|` ith_bitword64 n ctr;
+      par <- ith_bitword64 n (ctr + 1) `^` ith_bitword64 n ctr;
+      (x1,x2) <- if as_bool par then (x2,x1) else (x1, x2);
+      x1 <@ M.mulm(m,x1,x2); 
+      x2 <@ M.mulm(m,x2,x2);  
+      (x1,x3) <- as_bool (d `^` p) ? (x3,x1) : (x1,x3);
+      (x2,x4) <- as_bool (d `^` p)  ? (x4,x2) : (x2,x4);
+    }
+    (x1,x2) <- if ! as_bool (ith_bitword64 n 0)  then (x2,x1) else (x1, x2);    
+    return x1;
+  }  
+
+
+}.
+
+
+
+lemma exp_4_5' :
+ equiv[ M4.expm ~ M5.expm'  : ={arg} ==> ={res}].
+proc.
+inline ASpecFp.mulmw64.
+    wp.
+    wp.
+while (={ctr, n,  x1,x2,  x3, x4, d, p}).
+ wp. skip. progress. 
+wp.  
+skip. 
+progress.
+qed.
+
+
+
+
+lemma exp_4_5'' :
+ equiv[ M5.expm' ~ M5.expm  : arg{2}.`2 = arg{1}.`1 /\ arg{2}.`3 = arg{1}.`2 /\   ImplWord m{2} P ==> ={res}].
+symmetry.
+proc. 
+wp. 
+while (={ctr, n,  x1,x2,  x3, x4, d, p} /\ ImplWord m{1} P).
+ wp. 
+call mulm_specw64.
+call mulm_specw64. 
+wp. 
+skip. 
+progress.
+wp. 
+call mulm_specw64. 
+wp. 
+skip.
+progress.
+qed.
+
+
+
+
+
+
+
+
+
